lambda

Lambda.dfy
@@ -1,6 +1,6 @@
 include "objects.dfy"
-type Id= string 
-datatype LambdaTerm = Var(name:string) | Lambda(x:Id,t:LambdaTerm) | Application( t1:LambdaTerm, t2:LambdaTerm)
+type Id= nat
+datatype LambdaTerm = Var(id:Id) | Lambda(x:Id,t:LambdaTerm) | Application( t1:LambdaTerm, t2:LambdaTerm)
 
 function bound(t:LambdaTerm):seq<Id>
     ensures allUnique(bound(t))
@@ -10,16 +10,26 @@ function bound(t:LambdaTerm):seq<Id>
                 case Lambda(x,t) => addition(x,bound(t))
                 case Application(t1,t2) => reunion(bound(t1),bound(t2))
 }
+predicate includes(s1:seq<Id>,s2:seq<Id>)
+    
+{
+    forall id2:nat::id2<|s2| ==> (exists id1:nat::id1<|s1| && s1[id1]==s2[id2])
+}
 function addition(x:Id,s:seq<Id>) : seq<Id>
     requires allUnique(s)
     ensures var s':=addition(x,s);
-            allUnique(s') && x in s'
+            allUnique(s') && x in s' && includes(s',s)
+
 {
-    if x in s then s
-    else  assert !(x in s);
-        assert x in (s+[x]);
-        assert allUnique(s+[x]); 
-        s+[x]
+    if x in s 
+        then s
+    else  
+        assert !(x in s);
+        var s':=s+[x];
+        assert x in s';
+        assert allUnique(s');    
+        assert forall id:nat::id<|s| ==> s[id]==s'[id];
+        s'
 }
 function reunion(s1:seq<Id>,s2:seq<Id>) :seq<Id>
     requires allUnique(s1)
@@ -28,13 +38,37 @@ function reunion(s1:seq<Id>,s2:seq<Id>) :seq<Id>
         allUnique(s) 
         && (forall str:Id::str in s ==> (str in s1 || str in s2))
         && (forall str:Id::str in s1 || str in s2 ==> (str in s) )&&
-        |s| >= |s1| && |s| >= |s2|
+        |s| >= |s1| && |s| >= |s2| 
 {
     if s1==[] 
         then s2
     else
-
         [s1[0]]+reunion(remove(s1,s1[0]),remove(s2,s1[0]))
+}
+lemma reunionIncludesBothSets(s1:seq<Id>,s2:seq<Id>)
+    requires allUnique(s1)
+    requires allUnique(s2)
+    ensures var s:=reunion(s1,s2);
+    includes(s,s1) && includes(s,s2)
+{
+    var s:=reunion(s1,s2);
+    assert forall str:Id :: str in s1 ==> str in s;
+    assert forall str:Id :: str in s2 ==> str in s;
+
+    forall id2:nat | id2 < |s1|
+        ensures exists id1:nat :: id1 < |s| && s[id1] == s1[id2]
+    {
+        assert s1[id2] in s1;  
+        assert s1[id2] in s;   
+    }
+    assert forall id2:nat::id2<|s1| ==> (exists id1:nat::id1<|s| && s[id1]==s1[id2]);
+    forall id2:nat | id2 < |s2|
+        ensures exists id1:nat :: id1 < |s| && s[id1] == s2[id2]
+    {
+        assert s2[id2] in s2;
+        assert s2[id2] in s;
+    }
+    assert forall id2:nat::id2<|s2| ==> (exists id1:nat::id1<|s| && s[id1]==s2[id2]);
 }
 lemma elementNotInallUnique (s:seq<Id>,x:Id)
     requires !(x in s)
@@ -46,15 +80,20 @@ ghost predicate allUnique (s:seq<Id>)
 {
     forall id1:nat,id2:nat::(id1<id2<|s|) ==> s[id1]!=s[id2]
 }
-ghost predicate isGoodForWork(s:seq<Id>)
-    requires allUnique(s)
+predicate finds(s:seq<Id>,id:Id)
+    ensures finds(s,id) <==> exists id1:nat::id1<|s| && s[id1]==id
 {
-    forall str:Id:: ((str in s) && |str|>1 && str[0]=='n' && isStringAValidNumber(str[1..])) ==> stringToNat(str[1..])<|s|
+    if s==[] then false 
+        else 
+            if s[0]==id then true 
+                else finds(s[1..],id)
+
 }
+
 lemma reunionIsGoodForWork(s1:seq<Id>,s2:seq<Id>)
-    requires allUnique(s1) && isGoodForWork(s1)
-    requires allUnique(s2) && isGoodForWork(s2)
-    ensures allUnique(reunion(s1,s2)) && isGoodForWork(reunion(s1,s2))
+    requires allUnique(s1) 
+    requires allUnique(s2) 
+    ensures allUnique(reunion(s1,s2)) 
 {
     var s:=reunion(s1,s2);
     assert forall str:Id::(str in s1 || str in s2) ==> (str in s);
@@ -62,14 +101,36 @@ lemma reunionIsGoodForWork(s1:seq<Id>,s2:seq<Id>)
     assert |s|>=|s1|;
     assert |s|>=|s1| && |s|>=|s2|;
 }
-function addAnUniqueId(s:seq<Id>) : seq<Id>
-    requires allUnique(s) && isGoodForWork(s)
-    ensures allUnique(addAnUniqueId(s)) && isGoodForWork(addAnUniqueId(s))
+function max(a:nat,b:nat) :nat 
+    ensures var maxi:=max(a,b);
+    maxi>=a && maxi>=b && (maxi==a || maxi==b)
 {
-    var str:="n"+natToString(|s|);
-    natToStringThenStringToNatIdem(|s|);
-    assert !(str in s);
-    [str] +s
+    if a>b then a else b 
+}
+
+function highestId(s:seq<Id>) :nat
+    ensures s!=[] ==> forall index:nat:: index<|s| ==> s[index]<=highestId(s)
+    ensures s!=[] ==> exists index:nat:: index<|s| && s[index]==highestId(s)
+    ensures s==[] ==> highestId(s)==0
+    decreases s
+{
+        if s==[] then 0
+        else
+            max(s[0],highestId(s[1..]))
+}
+function addAnUniqueId(s:seq<Id>) :seq<Id>
+    requires allUnique(s)
+    ensures allUnique(addAnUniqueId(s))
+    ensures includes(addAnUniqueId(s),s)
+    ensures |addAnUniqueId(s)|==|s|+1
+    ensures !(addAnUniqueId(s)[0] in s)
+{
+    if s==[] then 
+        [0]
+    else
+        var s':= [highestId(s)+1]+s;
+        assert forall id:nat::id<|s| ==> s[id]==s'[id+1];
+        s'
 }
 function remove(s:seq<Id>,x:Id):seq<Id>
     requires allUnique(s) 
@@ -78,6 +139,7 @@ function remove(s:seq<Id>,x:Id):seq<Id>
     ensures forall str:Id:: str in remove(s,x) ==> str in s
     ensures forall str:Id:: str in s && str!=x ==> str in remove(s,x)
     ensures |s|-1<=|remove(s,x)|<=|s|
+    ensures includes(s,remove(s,x))
 {
     if s==[] then []
     else 
@@ -90,6 +152,7 @@ function remove(s:seq<Id>,x:Id):seq<Id>
         [s[0]]+remove(s[1..],x)
 
 }
+
 function free(t:LambdaTerm):seq<Id>
     ensures allUnique(free(t))
 {
@@ -107,35 +170,273 @@ function vars(t:LambdaTerm):seq<Id>
                 case Lambda(x,t') => addition(x,vars(t'))
                 case Application(t1,t2) => reunion(vars(t1),vars(t2))
 }
-function substitution(t:LambdaTerm,x:Id,t':LambdaTerm):LambdaTerm
+lemma varsOfALambdaIncludesVarsofASubLambda (t:LambdaTerm)
+    ensures var ids:=vars(t);
+    
+    match t
+                case Var(x) => x in ids 
+                case Lambda(x,t') => (x in ids) && includes(ids,vars(t'))
+                case Application(t1,t2) => includes(ids,vars(t1)) && includes(ids,vars(t2))
+{
+    var ids:=vars(t);
+
+    match t 
+         case Var(x) => assert ids==[x];
+                case Lambda(x,t') => assert ids==addition(x,vars(t'));
+                case Application(t1,t2) => {
+                    
+                    assert ids==reunion(vars(t1),vars(t2));
+                    reunionIncludesBothSets(vars(t1),vars(t2));
+                    
+                }
+}
+function lHeight(t:LambdaTerm):nat 
 {
     match t
-        case Var(y) => if y==x then t' else Var(y)
-        case Lambda(y,t1) => if y==x then t else   Lambda(y,substitution(t1,x,t'))
+                case Var(x) => 1
+                case Lambda(x,t') => 1+lHeight(t')
+                case Application(t1,t2) => 1+max(lHeight(t1),lHeight(t2))
+}
+function substitution(t:LambdaTerm,x:Id,t':LambdaTerm):LambdaTerm
+    decreases lHeight(t)
+{
+    match t
+        case Var(y) =>  if y==x 
+                            then 
+                            assert vars(t)<=reunion(vars(t),vars(t'));
+                            t' 
+                        else Var(y)
+        case Lambda(y,t1) =>    if y==x 
+                                    then 
+                                    
+                                    t 
+                                else   Lambda(y,substitution(t1,x,t'))
         case Application(t1,t2) => Application(substitution(t1,x,t'),substitution(t2,x,t'))
 }
 
 function caSubstitution(t:LambdaTerm,x:Id,t':LambdaTerm):LambdaTerm
     requires var s1:=vars(t);
-        allUnique(s1) && isGoodForWork(s1)
+        allUnique(s1) 
     requires var s2:=vars(t');
-        allUnique(s2) && isGoodForWork(s2)
-    ensures var s:=vars(caSubstitution(t,x,t'));
-        allUnique(s) && isGoodForWork(s)
+        allUnique(s2)
+
 {
+    var ids:=reunion(vars(t),vars(t'));
+    reunionIncludesBothSets(vars(t),vars(t'));
     caSubstitution'(t,x,t',reunion(vars(t),vars(t')))
+}
+lemma subsitutionOfVarDoesNotChangeHeightFORVARIABLES(t1:LambdaTerm,x:Id,t2:LambdaTerm)
+    requires match t2 
+                case Var(x) => true 
+                case _ => false 
+    ensures lHeight(substitution(t1,x,t2))==lHeight(t1)
+{
+    var t':=substitution(t1,x,t2);
+    match t1{
+        case Var(y) => {
+            assert lHeight(t')==lHeight(t1);
+            } 
+        case Lambda(y,t) => {if (y==x) {
+            assert t'==t1;
+    } else {
+        subsitutionOfVarDoesNotChangeHeightFORVARIABLES(t,x,t2);
+
+    }
+    }
+        case Application(t1,t2) => {
+
+        }
+    }
+}
+            
+lemma newIdsDueToSubstitution(t1:LambdaTerm,x:Id,t2:LambdaTerm,ids:seq<Id>)
+    requires includes(ids,vars(t1))
+    requires includes(ids,vars(t2))
+    ensures includes(ids,vars(substitution(t1,x,t2)))
+{
+    match t1
+        case Var(y) => {
+
+        }
+        case Lambda(y, t) => {
+            if y == x {
+            } else {
+                var t' := substitution(t, x, t2);
+
+                forall id2:nat | id2 < |vars(t)| 
+                    ensures vars(t)[id2] in ids 
+                {
+                    assert vars(t)[id2] in vars(t1); 
+                }
+
+                assert includes(ids, vars(t));
+
+                newIdsDueToSubstitution(t, x, t2, ids);
+
+                var new_vars := addition(y, vars(t'));
+                forall id2:nat | id2 < |new_vars|
+                    ensures new_vars[id2] in ids 
+                {
+                    var elem := new_vars[id2];
+                    if elem == y {
+                        assert y in vars(t1); 
+                    } else {
+                        assert elem in vars(t'); 
+                    }
+                }
+            }
+        }
+        case Application(t1', t2') => {
+            var sub_t1' := substitution(t1', x, t2);
+            var sub_t2' := substitution(t2', x, t2);
+
+            forall id2:nat | id2 < |vars(t1')| ensures vars(t1')[id2] in ids {
+                assert vars(t1')[id2] in vars(t1);
+            }
+            assert includes(ids, vars(t1'));
+
+            forall id2:nat | id2 < |vars(t2')| ensures vars(t2')[id2] in ids {
+                assert vars(t2')[id2] in vars(t1);
+            }
+            assert includes(ids, vars(t2'));
+
+            newIdsDueToSubstitution(t1', x, t2, ids);
+            newIdsDueToSubstitution(t2', x, t2, ids);
+
+            var new_vars := reunion(vars(sub_t1'), vars(sub_t2'));
+            forall id2:nat | id2 < |new_vars|
+                ensures new_vars[id2] in ids
+            {
+                var elem := new_vars[id2];
+                assert elem in vars(sub_t1') || elem in vars(sub_t2'); 
+            }
+        }
 }
 
 function caSubstitution'(t:LambdaTerm,x:Id,t':LambdaTerm,ids:seq<Id>):LambdaTerm
-    requires forall str:Id::str in reunion(vars(t),vars(t')) ==> str in ids 
-    requires allUnique(ids) && isGoodForWork(ids)
+    requires allUnique(ids)
+        requires var s1:=vars(t);
+         allUnique(s1) && includes(ids,s1)
+    requires var s2:=vars(t');
+         allUnique(s2)  && includes(ids,s2)
+    decreases lHeight(t)
 {
     match t
         case Var(y) => if y==x then t' else Var(y)
         case Lambda(y,t1) => if y==x then t else
-                                if !(y in free(t')) then Lambda(y,caSubstitution'(t,x,t',ids))
+                                if !(y in free(t')) then Lambda(y,caSubstitution'(t1,x,t',ids))
                                     else
-                                        var ids':=addAnUniqueId(ids);
-                                        Lambda(ids'[0],caSubstitution'())
-        case Application(t1,t2) => Application(substitution(t1,x,t'),substitution(t2,x,t'))
+                                         var ids':=addAnUniqueId(ids);
+                                            var vari:=Var(ids'[0]);
+                                         var t2:=substitution(t1,y,vari);
+                                         subsitutionOfVarDoesNotChangeHeightFORVARIABLES(t1,y,vari);
+                                         varsOfALambdaIncludesVarsofASubLambda (t);
+                                         newIdsDueToSubstitution(t1,y,vari,ids');
+                                         Lambda(ids'[0],
+                                         caSubstitution'(t2,x,t',ids'))
+        case Application(t1,t2) => 
+        varsOfALambdaIncludesVarsofASubLambda (t);
+        Application(caSubstitution'(t1,x,t',ids),caSubstitution'(t2,x,t',ids))
 }
+
+lemma CaSubstitution'OfVarDoesNotChangeHeight(t1:LambdaTerm, x:Id, t2:LambdaTerm, ids:seq<Id>)
+    requires match t2 case Var(_) => true case _ => false
+    requires allUnique(ids)
+    requires includes(ids,vars(t1)) && includes(ids,vars(t2))
+    ensures lHeight(caSubstitution'(t1, x, t2, ids)) == lHeight(t1)
+    decreases lHeight(t1)
+{
+    match t1 {
+        case Var(_) => {}
+        case Lambda(y, t1') => {
+            if y == x {
+            } else if !(y in free(t2)) {
+                CaSubstitution'OfVarDoesNotChangeHeight(t1', x, t2, ids);
+            } else {
+                // alpha-rename branch
+                var ids' := addAnUniqueId(ids);
+                var vari  := Var(ids'[0]);
+                var t2' := substitution(t1', y, vari);
+                subsitutionOfVarDoesNotChangeHeightFORVARIABLES(t1', y, vari);
+                 newIdsDueToSubstitution(t1',y,vari,ids');
+                CaSubstitution'OfVarDoesNotChangeHeight(t2', x, t2, ids');
+            }
+        }
+        case Application(t1', t1'') => {
+            varsOfALambdaIncludesVarsofASubLambda (t1);
+            CaSubstitution'OfVarDoesNotChangeHeight(t1', x, t2, ids);
+            CaSubstitution'OfVarDoesNotChangeHeight(t1'', x, t2, ids);
+        }
+    }
+}
+
+lemma CaSubsitutionOfVarDoesNotChangeHeightFORVARIABLES(t1:LambdaTerm, x:Id, t2:LambdaTerm)
+    requires match t2 case Var(_) => true case _ => false
+    ensures lHeight(caSubstitution(t1, x, t2)) == lHeight(t1)
+{
+    var ids := reunion(vars(t1), vars(t2));
+    reunionIncludesBothSets(vars(t1),vars(t2));
+    CaSubstitution'OfVarDoesNotChangeHeight(t1, x, t2, ids);
+}
+
+lemma ASubLambdaOfAUniqueLambdaIsUnique(t:LambdaTerm)
+    requires allUnique(vars(t))
+    ensures match t 
+                case Var(_)=> true 
+                case Application(t1,t2) => allUnique(vars(t1)) && allUnique(vars(t2))
+                case Lambda(_,t') => allUnique(vars(t'))
+{
+
+}
+
+function minim (a:nat,b:nat) : nat
+    ensures minim(a,b)<=a && minim(a,b)<=b
+    ensures minim(a,b)==a || minim(a,b)==b
+{
+    if a>b then b 
+    else a 
+}
+predicate alphaEquivalence(t1:LambdaTerm,t2:LambdaTerm)
+
+{
+    alphaEquivalence'(t1,t2,[],[])
+}
+function findId(ids:seq<Id>,id:Id):Option<nat>
+    decreases ids
+{
+    if ids==[] then None 
+        else 
+            var len:=|ids|;
+            if ids[len-1]==id then 
+                Some(len-1)
+            else 
+                findId(ids[..(len-1)],id)
+}   
+predicate alphaEquivalence'(t1:LambdaTerm,t2:LambdaTerm,id1:seq<Id>,id2:seq<Id>)
+    decreases minim(lHeight(t1),lHeight(t2))
+
+{
+    
+    match t1
+        case Var(x) => (match t2 
+                            case Var(y) => (
+                                var r1:=findId(id1,x);
+                                var r2:=findId(id2,y);
+                                r1==r2 
+                                &&
+                                match r1
+                                    case None => x==y
+                                    case Some(_) => true 
+                            )
+                            case _ => false
+                        ) 
+        case Lambda(x,t1') => (match t2
+                                case Lambda(y,t2') => 
+
+                                    alphaEquivalence'(t1',t2',id1+[x],id2+[y])
+                                case _=> false)
+        case Application(t1',t1'') => match t2
+                                        case Application(t2',t2'')=> alphaEquivalence'(t1',t2',id1,id2) && alphaEquivalence'(t1'',t2'',id1,id2)
+                                        case _=>false
+}
+
