BetaReduction.dfy
@@ -1,0 +1,82 @@
+include "Lambda.dfy"
+
+predicate isCorrectForBetaReduction(t:LambdaTerm)
+{
+    match t
+                case Application(Lambda(_,_),_) => true
+                case _ => false
+}
+
+function betaReduction(t:LambdaTerm) : LambdaTerm
+    requires isCorrectForBetaReduction(t)
+            
+{
+    match t 
+        case Application(Lambda(x,t1),t2) => caSubstitution(t1,x,t2)
+}
+
+function numberOfPossibleReducations (t:LambdaTerm) :nat 
+{
+    match t 
+        case Var(_) => 0
+        case Lambda(_,t') => numberOfPossibleReducations(t')
+        case Application(t1,t2) =>  if isCorrectForBetaReduction(t) then 1+numberOfPossibleReducations(t1)+numberOfPossibleReducations(t2)
+                                    else numberOfPossibleReducations(t1)+numberOfPossibleReducations(t2)
+}
+
+
+function betaReductionStep(t:LambdaTerm,choice:nat) : LambdaTerm
+    requires 0<numberOfPossibleReducations(t)
+    requires choice<numberOfPossibleReducations(t)
+{
+    if isCorrectForBetaReduction(t) then 
+        if choice==0 then
+            betaReduction(t)
+        else 
+            match t
+                case Application(t1,t2) => (
+                    var n1:=numberOfPossibleReducations(t1);
+                    if n1>=choice then
+                        assert choice<=n1;
+                        Application(betaReductionStep(t1,choice-1),t2)
+                    else 
+                        assert choice>n1;
+                        assert choice<numberOfPossibleReducations(t);
+                        assert numberOfPossibleReducations(t2)+n1+1==numberOfPossibleReducations(t);
+                        Application(t1,betaReductionStep(t2,choice-n1-1))
+                ) 
+    else 
+        match t
+                case Lambda(x,t')=> Lambda(x,betaReductionStep(t',choice))
+                case Application(t1,t2) => (
+                    var n1:=numberOfPossibleReducations(t1);
+                    if n1>choice then
+                        Application(betaReductionStep(t1,choice),t2)
+                    else 
+                        assert choice>=n1;
+                        assert choice<numberOfPossibleReducations(t);
+                        assert numberOfPossibleReducations(t2)+n1==numberOfPossibleReducations(t);
+                        Application(t1,betaReductionStep(t2,choice-n1))
+                )
+
+}
+
+predicate betaReductionClosure (t1:LambdaTerm,t2:LambdaTerm)
+{
+    exists n:nat::n<numberOfPossibleReducations(t1) && betaReductionStep(t1,n)==t2
+}
+
+
+ghost predicate betaReducationInNSteps (t1:LambdaTerm,t2:LambdaTerm,n:nat)
+    decreases n
+{
+    if n==0 then t1==t2 
+    else
+        exists t':LambdaTerm:: betaReductionClosure(t1,t')  && betaReducationInNSteps(t',t2,n-1)
+}
+
+ghost predicate betaReducationsClosure(t1:LambdaTerm,t2:LambdaTerm)
+{
+    exists n:nat:: betaReducationInNSteps(t1,t2,n)
+}
+// De a demonstra confluenta pe dabaz documentului de la waterloo https://student.cs.uwaterloo.ca/~cs442/W22/extras/c-r-thm-proof.pdf
