Confluence.dfy
@@ -1,0 +1,46 @@
+include "Lambda.dfy"
+include "BetaReduction.dfy"
+
+
+ghost predicate parallelReduction(t1:LambdaTerm,t2:LambdaTerm)
+    decreases lHeight(t1)
+{
+    match t1 
+            case Application(t1a,t1b) =>( match t2 
+                                        case Application(t2a,t2b) => parallelReduction(t1a,t2a) && parallelReduction(t1b,t2b)
+                                        case _ => false
+            ) ||
+            ( match t1a 
+                    case Lambda(x,M) => ( 
+                     exists M': LambdaTerm, N': LambdaTerm ::
+              assert lHeight(M)<lHeight(t1);       
+              parallelReduction(M, M')          
+              && parallelReduction(t1b, N')    
+              && t2 == substitution(M', x, N') 
+                    )
+                    case _=> t1==t2 
+            ) 
+            case Lambda(x,t1a) => (
+                ( match t2 
+                                        case Lambda(y,t2a)=> x==y && parallelReduction(t1a,t2a)
+                                        case _ => false
+            )
+            )
+            case _ => t1==t2
+}
+
+lemma parallelReductionIsReflexive (t:LambdaTerm)
+    ensures parallelReduction(t,t)
+{
+
+}
+
+
+// lemma SubstitutionLemma (M:LambdaTerm,N:LambdaTerm,P:LambdaTerm,x:Id,y:Id)
+//     requires x!=y
+//     requires !(x in free(P))
+//     ensures caSubstitution(caSubstitution(M,x,N),y,P)==caSubstitution(caSubstitution(M,y,P),x,caSubstitution(N,y,P))
+
+// {
+
+// }
